

# THE “ABRACADABRA” PROBLEM

FRANCESCO CARAVENNA

**ABSTRACT.** We present a detailed solution of Exercise E10.6 in [Wil91]: in a random sequence of letters, drawn independently and uniformly from the English alphabet, the expected time for the first appearance of the word “ABRACADABRA” is  $26^{11} + 26^4 + 26$ .

We adopt the conventions  $\mathbb{N} := \{1, 2, 3, \dots\}$  and  $\mathbb{N}_0 := \mathbb{N} \cup \{0\}$ .

## 1. FORMULATION OF THE PROBLEM

Let  $(U_i)_{i \in \mathbb{N}}$  denote random letters drawn independently and uniformly from the English alphabet. More precisely, we assume that  $(U_i)_{i \in \mathbb{N}}$  are independent and identically distributed random variables, uniformly distributed in the set  $\mathbf{E} := \{A, B, C, D, \dots, X, Y, Z\}$ , defined on some probability space  $(\Omega, \mathcal{A}, P)$ . For  $m, n \in \mathbb{N}$  with  $m \leq n$ , we use  $U_{[m,n]}$  as a shortcut for the vector  $(U_m, U_{m+1}, \dots, U_n)$ .

Define  $\tau$  as the random time in which the word “ABRACADABRA” first appears:

$$\tau := \min\{n \in \mathbb{N}, n \geq 11 : U_{[n-10,n]} = \text{ABRACADABRA}\}, \quad (1.1)$$

with the convention  $\min \emptyset := +\infty$ . Our goal is to prove the following result.

**Theorem 1.**  $E[\tau] = 26^{11} + 26^4 + 26$ .

## 2. STRATEGY

The proof is based on martingales. Let  $(\mathcal{F}_n)_{n \in \mathbb{N}_0}$  be the natural filtration of  $(U_i)_{i \in \mathbb{N}}$ , i.e.,  $\mathcal{F}_0 := \{\emptyset, \Omega\}$  and  $\mathcal{F}_n := \sigma(U_1, \dots, U_n)$ . We are going to prove the following results.

**Proposition 2.**  $\tau$  is a stopping time with  $E[\tau] < \infty$ .

**Proposition 3.** There exists a martingale  $M = (M_n)_{n \in \mathbb{N}_0}$  such that:

- (1)  $M_0 = 0$  and  $M_\tau = 26^{11} + 26^4 + 26 - \tau$ ;
- (2)  $M$  has bounded increments:  $\exists C \in (0, \infty)$  such that  $|M_{n+1} - M_n| \leq C$ , for all  $n \in \mathbb{N}_0$ .

Let us recall (a special case of) Doob’s optional sampling theorem, cf. [Wil91, §10.10].

**Theorem 4.** If  $M = (M_n)_{n \in \mathbb{N}_0}$  is a martingale with bounded increments and  $\tau$  is a stopping time with finite mean, then  $E[M_\tau] = E[M_0]$ .

Combining this with Propositions 2 and 3, one obtains immediately the proof of Theorem 1.

## 3. PROOF OF PROPOSITION 2

Recall that  $\tau$  is a stopping time if and only if  $\{\tau \leq n\} \in \mathcal{F}_n$  for every  $n \in \mathbb{N}_0$ . Note that  $\{\tau \leq n\} = \emptyset$  if  $n \leq 10$ , while for  $n \geq 11$

$$\{\tau \leq n\} = \bigcup_{i=11}^n \{U_{[i-10,i]} = \text{ABRACADABRA}\},$$

which shows that the event  $\{\tau \leq n\}$  is in  $\mathcal{F}_n$  (it is expressed as a function of  $U_1, U_2, \dots, U_n$ ).

To prove that  $E[\tau] < \infty$ , we argue as in [Wil91, §10.11; Exercise E10.5].

**Lemma 5.** *For a positive random variable  $\tau$ , in order to have  $E[\tau] < \infty$  it is sufficient that*

$$\exists N \in \mathbb{N}, \varepsilon > 0 : \quad P(\tau \leq n + N \mid \tau > n) \geq \varepsilon \quad \forall n \in \mathbb{N}_0. \quad (3.1)$$

This result is proved in Appendix A below. In order to apply it, let  $A_n$  be the event that the word “ABRACADABRA” appears (not necessarily for the first time!) at time  $n + 11$ :

$$A_n := \{U_{[n+1, n+11]} = \text{ABRACADABRA}\}.$$

By assumption  $U_i$  are independent and uniformly chosen letters, hence

$$P(A_n) = p^{11} > 0, \quad \text{where} \quad p := \frac{1}{E} = \frac{1}{26}.$$

Since  $A_n \subseteq \{\tau \leq n + 11\}$ , we have  $P(\tau \leq n + 11 \mid \tau > n) \geq P(A_n \mid \tau > n)$  for every  $n \in \mathbb{N}$ . However the events  $A_n$  and  $\{\tau > n\}$  are *independent* ( $A_n$  is a function of  $U_{[n+1, n+11]}$ , while  $\{\tau > n\} = \{\tau \leq n\}^c \in \mathcal{F}_n$  is a function of  $U_{[1, n]}$ ), hence  $P(A_n \mid \tau > n) = P(A_n)$ . Thus

$$P(\tau \leq n + 11 \mid \tau > n) \geq P(A_n) = p^{11},$$

i.e. relation (3.1) holds with  $N = 11$  and  $\varepsilon = p^{11}$ . It follows by Lemma 5 that  $E[\tau] < \infty$ .  $\square$

## 4. PROOF OF PROPOSITION 3

The required martingale  $M = (M_n)_{n \in \mathbb{N}_0}$  will be constructed as the total net gain of a suitable family of gamblers, built as follows.

At time 0 a first gambler enters the game, with an initial capital of 1€. She bets on the event that the first letter  $U_1$  is A (the first letter of the word “ABRACADABRA”). If she loses, her capital at time 1 drops to 0€ and she stops playing (i.e. her capital will stay 0€ at all later times). On the other hand, if she wins, her capital at time 1 becomes 26€ and she goes on playing, betting on the event that the second letter  $U_2$  is B (the second letter of “ABRACADABRA”). If she loses, her capital at time 2 is 0€ and she stops playing, while if she wins, her capital at time 2 equals  $(26)^2$ € and she goes on, betting on the event that the third letter  $U_3$  is R (the third letter of “ABRACADABRA”), and so on, until time 11.

The gambler’s capital at time 11 is either  $(26)^{11}$ €, if the letters  $U_{[1, 11]}$  have formed exactly the word “ABRACADABRA”, or 0€ otherwise. In any case, the gambler stops playing after time 11, hence her capital will stay constant at all later times.

Let us denote by  $x_i$  be the  $i$ -th letter of the word “ABRACADABRA”, for  $1 \leq i \leq 11$  (so that  $x_1 = A, x_2 = B, x_3 = R, \dots, x_{11} = A$ ). The capital (in €) of this first gambler at time  $n$  is then given by the process  $(K_n)_{n \in \mathbb{N}_0}$  defined as follows:

$$K_n := \begin{cases} 1 & \text{if } n = 0 \\ K_{n-1} \cdot 26 \mathbf{1}_{\{U_n = x_n\}} & \text{if } 1 \leq n \leq 11 \\ K_{11} & \text{if } n \geq 12 \end{cases}.$$

(Note that if  $K_{n-1} = 0$ , then  $K_n = 0$  irrespectively of  $U_n$ , as described above.)

Now a second gambler arrives, playing the same game, but with one time unit of delay. Her initial capital stays 1€ at time 0 and at time 1, then she bets on the event that  $U_2 = x_1 = A$ : if she loses, her capital at time 2 is 0€ and she stops playing, while if she wins, her capital at time 2 is 26€ and she goes on playing, betting on the event that  $U_3 = x_2 = B$ , etc. At time 12, the second gambler’s capital will be either  $(26)^{11}$ € or 0€, according to whether the letters  $U_{[2,12]}$  have formed precisely the word “ABRACADABRA” or not. At this point she stops playing and her capital stays constant at all later times.

Generalizing the picture, imagine that for each  $j \in \mathbb{N}$  there is a  $j$ -th gambler with an initial capital of 1€, who starts playing just before time  $j$ , betting on the event that  $U_j = x_1$ , then (if she wins) on  $U_{j+1} = x_2, \dots$ , and finally (if she has won all the previous bets) on  $U_{j+10} = x_{11}$ . After time  $j + 10$  the gambler stops playing and her capital stays constant.

Denoting by  $K_n^{(j)}$  the capital (in €) of the  $j$ -th gambler at time  $n$ , for  $n \in \mathbb{N}_0$ , we have

$$K_n^{(j)} := \begin{cases} 1 & \text{if } n < j \\ K_{n-1}^{(j)} \cdot 26 \mathbb{1}_{\{U_n = x_{(n-j)+1}\}} & \text{if } j \leq n \leq j + 10 \\ K_{j+10}^{(j)} & \text{if } n > j + 10 \end{cases} . \quad (4.1)$$

We can finally define the process we are looking for, that will be shown to be a martingale:

$$M_0 := 0, \quad M_n := \sum_{j=1}^n (K_n^{(j)} - K_0^{(j)}) = \left( \sum_{j=1}^n K_n^{(j)} \right) - n. \quad (4.2)$$

Thus  $M_n$  is the sum of the *net gains*  $K_n^{(j)} - K_0^{(j)}$  of the *first  $n$  gamblers* at time  $n$ .<sup>†</sup> For the equality in (4.2), recall that  $K_0^{(j)} = 1$  for all  $j \in \mathbb{N}$ .

**Lemma 6.** *For  $\tau$  defined as in (1.1), one has  $M_\tau = (26)^{11} + (26)^4 + 26 - \tau$ .*

*Proof.* We need to evaluate

$$M_\tau = \left( \sum_{j=1}^{\tau} K_\tau^{(j)} \right) - \tau.$$

Recall that  $K_\tau^{(j)}$  is the capital at time  $\tau$  of the gambler who starts betting just before time  $j$ . It suffices to show that  $K_\tau^{(j)} = 0$  except for  $j \in \{\tau - 10, \tau - 3, \tau\}$ , for which

$$K_\tau^{(\tau-10)} = (26)^{11}, \quad K_\tau^{(\tau-3)} = (26)^4, \quad K_\tau^{(\tau)} = 26.$$

Since the complete word “ABRACADABRA” appears at time  $\tau$ , the gambler who started playing just before time  $\tau - 10$  has a capital of  $(26)^{11}$ , i.e.  $K_\tau^{(\tau-10)} = (26)^{11}$ . The gambler who started playing just before time  $\tau - 3$  has a capital  $K_\tau^{(\tau-3)} = (26)^4$ , because the *last* four letters of “ABRACADABRA” are “ABRA” and coincide with the *first* four letters of that word. Analogously, since the last letter “A” is the same as the first letter, the gambler who started playing just before time  $\tau$  has won his first bet and his capital is  $K_\tau^{(\tau)} = 26$ .

Finally, for all  $j \notin \{\tau - 10, \tau - 3, \tau\}$  all gamblers have lost at least one bet and their capital is  $K_\tau^{(j)} = 0$ , because  $\tau$  is the *first* time the word “ABRACADABRA” appears.  $\square$

<sup>†</sup>We could have equivalently summed the net gains of *all* gamblers, defining  $M_n := \sum_{j=1}^{\infty} (K_n^{(j)} - K_0^{(j)})$ , because  $K_n^{(j)} = K_0^{(j)}$  for  $j > n$ .

To complete the proof of Proposition 3, it remains to show that  $M = (M_n)_{n \in \mathbb{N}_0}$  is a martingale with bounded increments. We start looking at the capital processes.

**Lemma 7.** *For every fixed  $j \in \mathbb{N}$ , the capital process  $(K_n^{(j)})_{n \in \mathbb{N}_0}$  is a martingale.*

*Proof.* We argue for fixed  $j \in \mathbb{N}$ . Plainly,  $K_0^{(j)} = 1$  is  $\mathcal{F}_0$ -measurable. By (4.1),  $K_n^{(j)}$  is a measurable function of  $K_{n-1}^{(j)}$  and  $U_n$ , assuming inductively that  $K_{n-1}^{(j)}$  is  $\mathcal{F}_{n-1}$ -measurable, it follows that  $K_n^{(j)}$  is  $\mathcal{F}_n$ -measurable. This shows that  $(K_n^{(j)})_{n \in \mathbb{N}_0}$  is an adapted process.

Since  $|K_n^{(j)}| \leq 26|K_{n-1}^{(j)}|$  by (4.1), it follows inductively that  $|K_n^{(j)}| \leq 26^n$  for all  $n \in \mathbb{N}$ , hence the random variables  $|K_n^{(j)}|$  are bounded (and, in particular, integrable).

Finally, the relation  $E[K_n^{(j)} | \mathcal{F}_{n-1}] = K_{n-1}^{(j)}$  is trivially satisfied if  $n < j$  or if  $n > j + 10$ , while for  $n \in \{j, \dots, j + 10\}$ , again by (4.1),

$$E[K_n^{(j)} | \mathcal{F}_{n-1}] = E[K_{n-1}^{(j)} \cdot 26 \mathbf{1}_{\{U_n = x_{(n-j)+1}\}} | \mathcal{F}_{n-1}] = K_{n-1}^{(j)} \cdot 26 P(U_n = x_{(n-j)+1}) = K_{n-1}^{(j)},$$

because  $U_n$  is independent of  $\mathcal{F}_{n-1}$  and  $P(U_n = a) = \frac{1}{26}$  for every  $a \in \mathbb{E}$ .  $\square$

**Lemma 8.** *The capital processes  $(K_n^{(j)})_{n \in \mathbb{N}_0}$  have uniformly bounded increments:*

$$|K_n^{(j)} - K_{n-1}^{(j)}| \leq 25^{11}, \quad \forall j, n \in \mathbb{N}. \quad (4.3)$$

*Proof.* One has  $|K_n^{(j)} - K_{n-1}^{(j)}| = 0$  if  $n < j$  or  $n > j + 10$ , by (4.1), while for  $n \in \{j, \dots, j + 10\}$

$$|K_n^{(j)} - K_{n-1}^{(j)}| \leq |26 \mathbf{1}_{\{U_n = x_{(n-j)+1}\}} - 1| |K_{n-1}^{(j)}| \leq 25 |K_{n-1}^{(j)}|.$$

Since  $K_{j-1}^{(j)} = 1$ , relation (4.3) follows.  $\square$

We can finally show that  $M$  is a martingale. Note that  $M_n$  is  $\mathcal{F}_n$ -measurable and in  $L^1$ , for every  $n \in \mathbb{N}$ , because by (4.2)  $M_n$  is a finite sum of  $K_n^{(j)}$ , each of which is  $\mathcal{F}_n$ -measurable and in  $L^1$  by Lemma 7. Furthermore, again by (4.2), for all  $n \in \mathbb{N}$  we can write

$$E[M_n | \mathcal{F}_{n-1}] = \sum_{j=1}^n E[K_n^{(j)} | \mathcal{F}_{n-1}] - n = \sum_{j=1}^n K_{n-1}^{(j)} - n.$$

However for  $j = n$  we have  $K_{n-1}^{(j)} = K_{n-1}^{(n)} = 1$  by definition, cf. (4.1), hence

$$E[M_n | \mathcal{F}_{n-1}] = \sum_{j=1}^{n-1} K_{n-1}^{(j)} + 1 - n = \sum_{j=1}^{n-1} K_{n-1}^{(j)} - (n-1) = M_{n-1}.$$

This shows that  $M$  is a martingale. Finally, for all  $n \in \mathbb{N}$

$$M_n - M_{n-1} = \sum_{j=1}^n K_n^{(j)} - n - \left( \sum_{j=1}^{n-1} K_{n-1}^{(j)} - (n-1) \right) = \sum_{j=1}^n (K_n^{(j)} - K_{n-1}^{(j)}),$$

again because for  $j = n$  we have  $K_{n-1}^{(j)} = K_{n-1}^{(n)} = 1$ . Now observe that, again by (4.1), for  $n \geq j + 11$  one has  $K_n^{(j)} = K_{n-1}^{(j)} = K_{j+10}^{(j)}$ , hence

$$|M_n - M_{n-1}| = \left| \sum_{j=n-10}^n (K_n^{(j)} - K_{n-1}^{(j)}) \right| \leq \sum_{j=n-10}^n |K_n^{(j)} - K_{n-1}^{(j)}| \leq 11 \cdot 25^{11},$$

having applied (4.3). This shows that  $M$  has bounded increments, completing the proof.  $\square$

## APPENDIX A. PROOF OF LEMMA 5

The assumptions imply that

$$P(\tau > \ell N) \leq (1 - \varepsilon)^\ell \quad \forall \ell \in \mathbb{N}_0, \quad (\text{A.1})$$

as we show below. We are going to use the formula

$$E[\tau] = \int_0^\infty P(\tau > t) dt, \quad (\text{A.2})$$

valid for every random variable  $\tau$  taking values in  $[0, \infty]$ .<sup>†</sup> Breaking up the integral in the sub-intervals  $[\ell N, (\ell + 1)N]$ , with  $\ell \in \mathbb{N}_0$ , since  $P(\tau > t) \leq P(\tau > \ell N)$  for  $t \geq \ell N$ , we get

$$\begin{aligned} E[\tau] &= \sum_{\ell \in \mathbb{N}_0} \int_{\ell N}^{(\ell+1)N} P(\tau > t) dt \leq \sum_{\ell \in \mathbb{N}_0} P(\tau > \ell N) \int_{\ell N}^{(\ell+1)N} 1 dt \leq \sum_{\ell \in \mathbb{N}_0} (1 - \varepsilon)^\ell N \\ &= \frac{N}{1 - (1 - \varepsilon)} = \frac{N}{\varepsilon} < \infty, \end{aligned}$$

having applied the geometric series  $\sum_{n \in \mathbb{N}_0} q^n = \frac{1}{1-q}$ . This shows that  $E[\tau] < \infty$ , as required.

It remains to prove (A.1), which we do by induction. For  $\ell = 0$  there is nothing to prove. For every  $\ell \in \mathbb{N}_0$ , since  $\{\tau > (\ell + 1)N\} \subseteq \{\tau > \ell N\}$ , we can write

$$\begin{aligned} P(\tau > (\ell + 1)N) &= P(\tau > (\ell + 1)N, \tau > \ell N) \\ &= P(\tau > \ell N) P(\tau > (\ell + 1)N \mid \tau > \ell N). \end{aligned} \quad (\text{A.3})$$

The induction step yields  $P(\tau > \ell N) \leq (1 - \varepsilon)^\ell$ , while assumption (3.1) gives

$$P(\tau > n + N \mid \tau > n) \leq (1 - \varepsilon), \quad \forall n \in \mathbb{N}.$$

Choosing  $n = \ell N$  yields  $P(\tau > (\ell + 1)N \mid \tau > \ell N) \leq (1 - \varepsilon)$ , which plugged into (A.3) yields  $P(\tau > (\ell + 1)N) \leq (1 - \varepsilon)^{\ell+1}$ , as required.  $\square$

## REFERENCES

[Wil91] D. Williams (1991), *Probability with martingales*, Cambridge University Press

DIPARTIMENTO DI MATEMATICA E APPLICAZIONI, UNIVERSITÀ DEGLI STUDI DI MILANO-BICOCCA, VIA COZZI 55, 20125 MILANO, ITALY

E-mail address: francesco.caravenna@unimib.it

---

<sup>†</sup>For every  $T \in [0, \infty]$  one has  $T = \int_0^T 1 dt = \int_0^\infty \mathbf{1}_{\{T \geq t\}} dt$ , hence  $\tau(\omega) = \int_0^\infty \mathbf{1}_{\{\tau(\omega) > t\}} dt$  for every random variable  $\tau$  taking values in  $[0, \infty]$ . Taking expectations of both sides and exchanging the expectation with the integral (which is justified by Fubini-Tonelli, thanks to positivity) one obtains (A.2).